solvers/95.lean
@@ -75,12 +75,12 @@ example :
   native_decide
 
 
-def solve (_n : Nat) :=
-  (amicableChainBest 1000000).2
+def solve (limit : Nat) :=
+  (amicableChainBest limit).2
 
-theorem equiv (n : Nat) : ProjectEulerStatements.P95.naive n n = solve n := sorry
+theorem equiv (limit : Nat) : ProjectEulerStatements.P95.naive limit = solve limit := sorry
 end ProjectEulerSolutions.P95
 open ProjectEulerSolutions.P95
 
 def main : IO Unit := do
-  IO.println (solve 0)
+  IO.println (solve 1000000)
